generational/spec/GC.Gen.CheneyBFS.fst
@@ -14,6 +14,7 @@ open GC.Gen.Promote
 open GC.Gen.Reachability
 
 module CheneySpec = GC.Gen.Cheney
+module SimOne = GC.Gen.Cheney.SimOne
 
 /// ---------------------------------------------------------------------------
 /// Graph lemma: fwd_well_formed ⟹ all reachable forwarded
@@ -32,19 +33,17 @@ let fwd_well_formed_covers_reachable
             minor_wosize minor x > 0 ==>
             fwd x <> 0UL)
   =
-  // Predicate: "if wosize > 0, then forwarded"
-  let p (x: U64.t) : prop = minor_wosize minor x > 0 ==> fwd x <> 0UL in
-  // Closure: if p(a) and b ∈ successors(a), then p(b)
-  // Two cases for a:
-  //   - wosize(a) > 0: p(a) gives fwd(a)≠0, fwd_closed gives fwd(b)≠0 if wosize(b)>0
-  //   - wosize(a) = 0: successors(a) is empty (length ≤ wosize = 0), contradiction
+  let p (x: U64.t) : prop =
+    Seq.mem x (minor_objects minor) /\ (minor_wosize minor x > 0 ==> fwd x <> 0UL) in
   let closure (a b: U64.t)
     : Lemma (requires p a /\ Seq.mem b (minor_successors minor a))
             (ensures p b)
-    = minor_successors_length minor a;
-      if minor_wosize minor a > 0
-      then () // fwd_closed handles this
-      else () // |successors| <= wosize = 0, but mem b => |successors| > 0, contradiction
+    =
+      let _i = Seq.index_mem b (minor_successors minor a) in
+      minor_successors_length minor a;
+      assert (minor_wosize minor a > 0);
+      assert (fwd a <> 0UL);
+      minor_successors_valid minor a b
   in
   Classical.forall_intro_2 (fun a -> Classical.move_requires (closure a));
   let aux (x: U64.t)
@@ -153,6 +152,7 @@ let rec scan_fwd_monotone
   if fuel = 0 || scan >= Seq.length cs.cs_queue then
     CheneySpec.cheney_scan_base minor cs scan fuel
   else begin
+    assert (fuel > 0);
     CheneySpec.cheney_scan_step minor cs scan fuel;
     let obj = Seq.index cs.cs_queue scan in
     let wz = minor_wosize minor obj in
@@ -161,11 +161,427 @@ let rec scan_fwd_monotone
     scan_fwd_monotone minor cs' (scan + 1) (fuel - 1) x
   end
 
+let scan_preserves_fwd_covers_roots
+  (minor: minor_state) (cs: CheneySpec.cheney_state)
+  (roots: seq U64.t) (scan fuel: nat)
+  : Lemma (requires minor_infix_wf minor /\
+                    fwd_covers_roots minor cs.cs_fwd roots)
+          (ensures fwd_covers_roots minor
+            (CheneySpec.cheney_scan minor cs scan fuel).cs_fwd roots)
+  =
+    let aux (r: U64.t) : Lemma
+      (requires Seq.mem r roots /\
+                Seq.mem r (minor_objects minor) /\
+                minor_wosize minor r > 0)
+      (ensures (CheneySpec.cheney_scan minor cs scan fuel).cs_fwd r <> 0UL)
+    =
+      assert (cs.cs_fwd r <> 0UL);
+      scan_fwd_monotone minor cs scan fuel r
+    in
+    FStar.Classical.forall_intro (FStar.Classical.move_requires aux)
+
+#pop-options
+
+#push-options "--z3rlimit 40 --fuel 1 --ifuel 0"
+let forward_one_queue_prefix
+  (minor: minor_state) (cs: CheneySpec.cheney_state) (addr: U64.t) (k: nat)
+  : Lemma (requires k < Seq.length cs.cs_queue)
+          (ensures k < Seq.length (CheneySpec.cheney_forward_one minor cs addr).cs_queue /\
+                   Seq.index (CheneySpec.cheney_forward_one minor cs addr).cs_queue k ==
+                   Seq.index cs.cs_queue k)
+  =
+    if cs.cs_fwd addr <> 0UL then
+      CheneySpec.cheney_forward_one_noop minor cs addr
+    else if is_infix_in_minor minor addr then begin
+      CheneySpec.cheney_forward_one_infix minor cs addr;
+      let parent = infix_parent minor addr in
+      let csn = CheneySpec.cheney_forward_normal minor cs parent in
+      if not (Seq.mem parent (minor_objects minor)) || cs.cs_fwd parent <> 0UL then
+        CheneySpec.cheney_forward_normal_noop minor cs parent
+      else if minor_wosize minor parent = 0 then
+        CheneySpec.cheney_forward_normal_noop_wz0 minor cs parent
+      else begin
+        let res = promote_object minor cs.cs_major parent cs.cs_fp (minor_wosize minor parent) in
+        if res.new_addr = 0UL then
+          CheneySpec.cheney_forward_normal_noop_oom minor cs parent
+        else begin
+          CheneySpec.cheney_forward_normal_success minor cs parent;
+          Seq.Base.lemma_index_app1 cs.cs_queue (Seq.create 1 parent) k
+        end
+      end
+    end else begin
+      CheneySpec.cheney_forward_one_normal minor cs addr;
+      if not (Seq.mem addr (minor_objects minor)) || cs.cs_fwd addr <> 0UL then
+        CheneySpec.cheney_forward_normal_noop minor cs addr
+      else if minor_wosize minor addr = 0 then
+        CheneySpec.cheney_forward_normal_noop_wz0 minor cs addr
+      else begin
+        let res = promote_object minor cs.cs_major addr cs.cs_fp (minor_wosize minor addr) in
+        if res.new_addr = 0UL then
+          CheneySpec.cheney_forward_normal_noop_oom minor cs addr
+        else begin
+          CheneySpec.cheney_forward_normal_success minor cs addr;
+          Seq.Base.lemma_index_app1 cs.cs_queue (Seq.create 1 addr) k
+        end
+      end
+    end
+
+let rec forward_fields_queue_prefix
+  (minor: minor_state) (cs: CheneySpec.cheney_state)
+  (parent: U64.t) (idx: nat) (wosize: nat) (k: nat)
+  : Lemma (requires k < Seq.length cs.cs_queue)
+          (ensures k < Seq.length (CheneySpec.cheney_forward_fields minor cs parent idx wosize).cs_queue /\
+                   Seq.index (CheneySpec.cheney_forward_fields minor cs parent idx wosize).cs_queue k ==
+                   Seq.index cs.cs_queue k)
+          (decreases (if idx < wosize then wosize - idx else 0))
+  =
+    if idx >= wosize then
+      CheneySpec.cheney_forward_fields_base minor cs parent idx wosize
+    else begin
+      CheneySpec.cheney_forward_fields_step minor cs parent idx wosize;
+      let child = to_minor_offset (minor_read_field minor parent idx) in
+      let cs' = CheneySpec.cheney_forward_one minor cs child in
+      forward_one_queue_prefix minor cs child k;
+      assert (k < Seq.length cs'.cs_queue);
+      forward_fields_queue_prefix minor cs' parent (idx + 1) wosize k
+    end
+#pop-options
+
+[@@"opaque_to_smt"]
+let addr_covered (minor: minor_state) (cs: CheneySpec.cheney_state) (addr: U64.t) : prop =
+  Seq.mem addr (minor_objects minor) /\ minor_wosize minor addr > 0 ==>
+  cs.cs_fwd addr <> 0UL
+
+#push-options "--z3rlimit 40 --fuel 0 --ifuel 0"
+let addr_covered_intro
+  (minor: minor_state) (cs: CheneySpec.cheney_state) (addr: U64.t)
+  : Lemma (requires (Seq.mem addr (minor_objects minor) /\
+                     minor_wosize minor addr > 0 ==> cs.cs_fwd addr <> 0UL))
+          (ensures addr_covered minor cs addr)
+  = reveal_opaque (`%addr_covered) (addr_covered minor cs addr)
+
+let addr_covered_elim
+  (minor: minor_state) (cs: CheneySpec.cheney_state) (addr: U64.t)
+  : Lemma (requires addr_covered minor cs addr /\
+                    Seq.mem addr (minor_objects minor) /\ minor_wosize minor addr > 0)
+          (ensures cs.cs_fwd addr <> 0UL)
+  = reveal_opaque (`%addr_covered) (addr_covered minor cs addr)
+
+let forward_one_preserves_addr_covered
+  (minor: minor_state) (cs: CheneySpec.cheney_state) (step_addr x: U64.t)
+  : Lemma (requires minor_infix_wf minor /\ addr_covered minor cs x)
+          (ensures addr_covered minor (CheneySpec.cheney_forward_one minor cs step_addr) x)
+  =
+    reveal_opaque (`%addr_covered) (addr_covered minor cs x);
+    reveal_opaque (`%addr_covered)
+      (addr_covered minor (CheneySpec.cheney_forward_one minor cs step_addr) x);
+    if Seq.mem x (minor_objects minor) && minor_wosize minor x > 0 then
+      forward_one_fwd_monotone minor cs step_addr x
+#pop-options
+
+[@@"opaque_to_smt"]
+let root_prefix_covered
+  (minor: minor_state) (cs: CheneySpec.cheney_state) (roots: seq U64.t) (idx: nat) : prop =
+  forall (j:nat). j < idx /\ j < Seq.length roots ==> addr_covered minor cs (Seq.index roots j)
+
+#push-options "--z3rlimit 40 --fuel 0 --ifuel 0"
+let root_prefix_empty (minor: minor_state) (cs: CheneySpec.cheney_state) (roots: seq U64.t)
+  : Lemma (ensures root_prefix_covered minor cs roots 0)
+  = reveal_opaque (`%root_prefix_covered) (root_prefix_covered minor cs roots 0)
+
+let root_prefix_step
+  (minor: minor_state) (cs: CheneySpec.cheney_state) (roots: seq U64.t) (idx: nat)
+  : Lemma (requires idx < Seq.length roots /\
+                    minor_infix_wf minor /\
+                    root_prefix_covered minor cs roots idx /\
+                    addr_covered minor (CheneySpec.cheney_forward_one minor cs (Seq.index roots idx))
+                      (Seq.index roots idx))
+          (ensures root_prefix_covered minor
+                    (CheneySpec.cheney_forward_one minor cs (Seq.index roots idx))
+                    roots (idx + 1))
+  =
+    let r = Seq.index roots idx in
+    let cs' = CheneySpec.cheney_forward_one minor cs r in
+    reveal_opaque (`%root_prefix_covered) (root_prefix_covered minor cs roots idx);
+    reveal_opaque (`%root_prefix_covered) (root_prefix_covered minor cs' roots (idx + 1));
+    let aux (j:nat{j < idx + 1 /\ j < Seq.length roots})
+      : Lemma (addr_covered minor cs' (Seq.index roots j))
+      =
+        if j = idx then ()
+        else begin
+          assert (j < idx);
+          forward_one_preserves_addr_covered minor cs r (Seq.index roots j)
+        end
+    in
+    FStar.Classical.forall_intro aux
+
+let root_prefix_step_oom
+  (minor: minor_state) (cs: CheneySpec.cheney_state) (roots: seq U64.t) (idx: nat)
+  (oom_before oom_after: bool)
+  : Lemma (requires idx < Seq.length roots /\
+                    minor_infix_wf minor /\
+                    (oom_before == true ==> oom_after == true) /\
+                    (not oom_before ==> root_prefix_covered minor cs roots idx) /\
+                    (not oom_after ==> addr_covered minor
+                      (CheneySpec.cheney_forward_one minor cs (Seq.index roots idx))
+                      (Seq.index roots idx)))
+          (ensures not oom_after ==> root_prefix_covered minor
+                    (CheneySpec.cheney_forward_one minor cs (Seq.index roots idx))
+                    roots (idx + 1))
+  =
+    if not oom_after then begin
+      assert (not oom_before);
+      root_prefix_step minor cs roots idx
+    end
+
+let root_prefix_all_implies_covers
+  (minor: minor_state) (cs: CheneySpec.cheney_state) (roots: seq U64.t)
+  : Lemma (requires root_prefix_covered minor cs roots (Seq.length roots))
+          (ensures fwd_covers_roots minor cs.cs_fwd roots)
+  =
+    reveal_opaque (`%root_prefix_covered)
+      (root_prefix_covered minor cs roots (Seq.length roots));
+    let aux (r:U64.t)
+      : Lemma (requires Seq.mem r roots /\ Seq.mem r (minor_objects minor) /\ minor_wosize minor r > 0)
+              (ensures cs.cs_fwd r <> 0UL)
+      =
+        let j = Seq.index_mem r roots in
+        assert (j < Seq.length roots);
+        assert (Seq.index roots j == r);
+        addr_covered_elim minor cs r
+    in
+    FStar.Classical.forall_intro (FStar.Classical.move_requires aux)
+
+let root_prefix_all_implies_covers_oom
+  (minor: minor_state) (cs: CheneySpec.cheney_state) (roots: seq U64.t) (oom: bool)
+  : Lemma (requires (not oom ==> root_prefix_covered minor cs roots (Seq.length roots)))
+          (ensures not oom ==> fwd_covers_roots minor cs.cs_fwd roots)
+  =
+    if not oom then root_prefix_all_implies_covers minor cs roots
+#pop-options
+
+[@@"opaque_to_smt"]
+let field_prefix_covered
+  (minor: minor_state) (cs: CheneySpec.cheney_state) (parent: U64.t) (idx: nat) : prop =
+  forall (j:nat). j < idx ==> addr_covered minor cs (to_minor_offset (minor_read_field minor parent j))
+
+#push-options "--z3rlimit 60 --fuel 0 --ifuel 0"
+let field_prefix_empty (minor: minor_state) (cs: CheneySpec.cheney_state) (parent: U64.t)
+  : Lemma (ensures field_prefix_covered minor cs parent 0)
+  = reveal_opaque (`%field_prefix_covered) (field_prefix_covered minor cs parent 0)
+
+let field_prefix_step
+  (minor: minor_state) (cs: CheneySpec.cheney_state) (parent: U64.t) (idx: nat)
+  : Lemma (requires minor_infix_wf minor /\
+                    field_prefix_covered minor cs parent idx /\
+                    addr_covered minor
+                      (CheneySpec.cheney_forward_one minor cs
+                        (to_minor_offset (minor_read_field minor parent idx)))
+                      (to_minor_offset (minor_read_field minor parent idx)))
+          (ensures field_prefix_covered minor
+                    (CheneySpec.cheney_forward_one minor cs
+                      (to_minor_offset (minor_read_field minor parent idx)))
+                    parent (idx + 1))
+  =
+    let child = to_minor_offset (minor_read_field minor parent idx) in
+    let cs' = CheneySpec.cheney_forward_one minor cs child in
+    reveal_opaque (`%field_prefix_covered) (field_prefix_covered minor cs parent idx);
+    reveal_opaque (`%field_prefix_covered) (field_prefix_covered minor cs' parent (idx + 1));
+    let aux (j:nat{j < idx + 1}) : Lemma (addr_covered minor cs' (to_minor_offset (minor_read_field minor parent j)))
+      =
+        if j = idx then ()
+        else begin
+          assert (j < idx);
+          forward_one_preserves_addr_covered minor cs child (to_minor_offset (minor_read_field minor parent j))
+        end
+    in
+    FStar.Classical.forall_intro aux
+
+let field_prefix_step_oom
+  (minor: minor_state) (cs: CheneySpec.cheney_state) (parent: U64.t) (idx: nat)
+  (oom_before oom_after: bool)
+  : Lemma (requires minor_infix_wf minor /\
+                    (oom_before == true ==> oom_after == true) /\
+                    (not oom_before ==> field_prefix_covered minor cs parent idx) /\
+                    (not oom_after ==> addr_covered minor
+                      (CheneySpec.cheney_forward_one minor cs
+                        (to_minor_offset (minor_read_field minor parent idx)))
+                      (to_minor_offset (minor_read_field minor parent idx))))
+          (ensures not oom_after ==> field_prefix_covered minor
+                    (CheneySpec.cheney_forward_one minor cs
+                      (to_minor_offset (minor_read_field minor parent idx)))
+                    parent (idx + 1))
+  =
+    if not oom_after then begin
+      assert (not oom_before);
+      field_prefix_step minor cs parent idx
+    end
+
+let field_prefix_all_implies_successors
+  (minor: minor_state) (cs: CheneySpec.cheney_state) (parent: U64.t)
+  : Lemma (requires field_prefix_covered minor cs parent (minor_wosize minor parent))
+          (ensures forall (y: U64.t).
+            Seq.mem y (minor_successors minor parent) /\
+            minor_wosize minor y > 0 ==> cs.cs_fwd y <> 0UL)
+  =
+    reveal_opaque (`%field_prefix_covered)
+      (field_prefix_covered minor cs parent (minor_wosize minor parent));
+    let aux (y: U64.t) : Lemma
+      (requires Seq.mem y (minor_successors minor parent) /\ minor_wosize minor y > 0)
+      (ensures cs.cs_fwd y <> 0UL)
+    =
+      minor_successors_char minor parent y;
+      let j = FStar.IndefiniteDescription.indefinite_description_ghost nat
+        (fun j -> j < minor_wosize minor parent /\
+                  to_minor_offset (minor_read_field minor parent j) == y /\
+                  is_minor_addr y /\ Seq.mem y (minor_objects minor)) in
+      assert (j < minor_wosize minor parent);
+      assert (to_minor_offset (minor_read_field minor parent j) == y);
+      addr_covered_elim minor cs y
+    in
+    FStar.Classical.forall_intro (FStar.Classical.move_requires aux)
+#pop-options
+
+[@@"opaque_to_smt"]
+let scanned_prefix_closed
+  (minor: minor_state) (cs: CheneySpec.cheney_state) (scan: nat) : prop =
+  forall (k:nat) (y:U64.t).
+    k < scan /\ k < Seq.length cs.cs_queue /\
+    Seq.mem y (minor_successors minor (Seq.index cs.cs_queue k)) /\
+    minor_wosize minor y > 0 ==> cs.cs_fwd y <> 0UL
+
+#push-options "--z3rlimit 80 --fuel 0 --ifuel 0"
+let scanned_prefix_empty
+  (minor: minor_state) (cs: CheneySpec.cheney_state)
+  : Lemma (ensures scanned_prefix_closed minor cs 0)
+  = reveal_opaque (`%scanned_prefix_closed) (scanned_prefix_closed minor cs 0)
+
+let scanned_prefix_step
+  (minor: minor_state) (cs cs': CheneySpec.cheney_state) (scan: nat)
+  : Lemma
+    (requires
+      minor_infix_wf minor /\
+      scanned_prefix_closed minor cs scan /\
+      scan < Seq.length cs.cs_queue /\
+      cs' == CheneySpec.cheney_forward_fields minor cs
+        (Seq.index cs.cs_queue scan) 0
+        (minor_wosize minor (Seq.index cs.cs_queue scan)) /\
+      field_prefix_covered minor cs'
+        (Seq.index cs.cs_queue scan)
+        (minor_wosize minor (Seq.index cs.cs_queue scan)))
+    (ensures scanned_prefix_closed minor cs' (scan + 1))
+  =
+    let parent = Seq.index cs.cs_queue scan in
+    reveal_opaque (`%scanned_prefix_closed) (scanned_prefix_closed minor cs scan);
+    reveal_opaque (`%scanned_prefix_closed) (scanned_prefix_closed minor cs' (scan + 1));
+    let aux (k:nat) (y:U64.t) : Lemma
+      (requires k < scan + 1 /\ k < Seq.length cs'.cs_queue /\
+                Seq.mem y (minor_successors minor (Seq.index cs'.cs_queue k)) /\
+                minor_wosize minor y > 0)
+      (ensures cs'.cs_fwd y <> 0UL)
+    =
+      if k = scan then begin
+        forward_fields_queue_prefix minor cs parent 0 (minor_wosize minor parent) scan;
+        assert (Seq.index cs'.cs_queue k == parent);
+        field_prefix_all_implies_successors minor cs' parent
+      end else begin
+        assert (k < scan);
+        assert (k < Seq.length cs.cs_queue);
+        forward_fields_queue_prefix minor cs parent 0 (minor_wosize minor parent) k;
+        assert (Seq.index cs'.cs_queue k == Seq.index cs.cs_queue k);
+        assert (cs.cs_fwd y <> 0UL);
+        forward_fields_fwd_monotone minor cs parent 0 (minor_wosize minor parent) y
+      end
+    in
+    FStar.Classical.forall_intro_2 (FStar.Classical.move_requires_2 aux)
+
+let scanned_prefix_step_oom
+  (minor: minor_state) (cs cs': CheneySpec.cheney_state) (scan: nat)
+  (oom_before oom_after: bool)
+  : Lemma
+    (requires
+      minor_infix_wf minor /\
+      (oom_before == true ==> oom_after == true) /\
+      (not oom_before ==> scanned_prefix_closed minor cs scan) /\
+      scan < Seq.length cs.cs_queue /\
+      cs' == CheneySpec.cheney_forward_fields minor cs
+        (Seq.index cs.cs_queue scan) 0
+        (minor_wosize minor (Seq.index cs.cs_queue scan)) /\
+      (not oom_after ==> field_prefix_covered minor cs'
+        (Seq.index cs.cs_queue scan)
+        (minor_wosize minor (Seq.index cs.cs_queue scan))))
+    (ensures not oom_after ==> scanned_prefix_closed minor cs' (scan + 1))
+  =
+    if not oom_after then begin
+      assert (not oom_before);
+      scanned_prefix_step minor cs cs' scan
+    end
+
+let scanned_exhausted_implies_fwd_closed
+  (minor: minor_state) (cs: CheneySpec.cheney_state) (scan: nat)
+  : Lemma (requires SimOne.cheney_bfs_inv minor cs /\
+                    scanned_prefix_closed minor cs scan /\
+                    scan >= Seq.length cs.cs_queue)
+          (ensures fwd_closed minor cs.cs_fwd)
+  =
+    SimOne.cheney_bfs_inv_fwd_in_queue minor cs;
+    reveal_opaque (`%scanned_prefix_closed) (scanned_prefix_closed minor cs scan);
+    let aux (x y: U64.t) : Lemma
+      (requires Seq.mem x (minor_objects minor) /\
+                cs.cs_fwd x <> 0UL /\
+                Seq.mem y (minor_successors minor x) /\
+                minor_wosize minor y > 0)
+      (ensures cs.cs_fwd y <> 0UL)
+    =
+      assert (Seq.mem x cs.cs_queue);
+      let k = Seq.index_mem x cs.cs_queue in
+      assert (k < Seq.length cs.cs_queue);
+      assert (k < scan);
+      assert (Seq.index cs.cs_queue k == x);
+      assert (Seq.mem y (minor_successors minor (Seq.index cs.cs_queue k)));
+      assert (cs.cs_fwd y <> 0UL)
+    in
+    FStar.Classical.forall_intro_2 (FStar.Classical.move_requires_2 aux)
+
+let scanned_exhausted_implies_fwd_closed_oom
+  (minor: minor_state) (cs: CheneySpec.cheney_state) (scan: nat) (oom: bool)
+  : Lemma (requires SimOne.cheney_bfs_inv minor cs /\
+                    (not oom ==> scanned_prefix_closed minor cs scan) /\
+                    scan >= Seq.length cs.cs_queue)
+          (ensures not oom ==> fwd_closed minor cs.cs_fwd)
+  =
+    if not oom then scanned_exhausted_implies_fwd_closed minor cs scan
 #pop-options
 
 /// ---------------------------------------------------------------------------
 /// Main theorem: BFS completeness under no-OOM
 /// ---------------------------------------------------------------------------
+
+let cheney_no_oom_from_loop_posts
+  (minor: minor_state) (major: heap) (fp: U64.t) (roots: seq U64.t)
+  (oom_roots oom_final: bool)
+  : Lemma (requires minor_infix_wf minor /\
+                    (let cs0 : CheneySpec.cheney_state =
+                       { CheneySpec.cs_major = major; CheneySpec.cs_fp = fp;
+                         CheneySpec.cs_fwd = empty_forwarding; CheneySpec.cs_queue = Seq.empty } in
+                     let cs1 = CheneySpec.cheney_forward_roots minor cs0 roots 0 in
+                     let cs2 = CheneySpec.cheney_scan minor cs1 0 (CheneySpec.cheney_fuel minor) in
+                     (oom_roots == true ==> oom_final == true) /\
+                     (not oom_roots ==> fwd_covers_roots minor cs1.CheneySpec.cs_fwd roots) /\
+                     (not oom_final ==> fwd_closed minor cs2.CheneySpec.cs_fwd)))
+          (ensures not oom_final ==> cheney_no_oom minor major fp roots)
+  =
+    if not oom_final then begin
+      let cs0 : CheneySpec.cheney_state =
+        { CheneySpec.cs_major = major; CheneySpec.cs_fp = fp;
+          CheneySpec.cs_fwd = empty_forwarding; CheneySpec.cs_queue = Seq.empty } in
+      let cs1 = CheneySpec.cheney_forward_roots minor cs0 roots 0 in
+      let cs2 = CheneySpec.cheney_scan minor cs1 0 (CheneySpec.cheney_fuel minor) in
+      assert (not oom_roots);
+      scan_preserves_fwd_covers_roots minor cs1 roots 0 (CheneySpec.cheney_fuel minor);
+      assert (fwd_well_formed minor cs2.CheneySpec.cs_fwd roots);
+      assert (cheney_no_oom minor major fp roots)
+    end
 
 let cheney_promotes_all_reachable
   (minor: minor_state) (major: heap) (fp: U64.t) (roots: seq U64.t)
